\begin{problem}{1} The posterior density can be found with Baye's rule:
\begin{equation*}
f_{X|Y}(x|2) = \frac{P_{Y|X}(2|x)f_X(x)}{\int P_{Y|X}(2|x)f_X(x)dx},
\end{equation*}
where
\begin{equation*}
P_{Y|X}(2|x) = x(1-x).
\end{equation*}
I therefore have that:
\begin{align*}
f_{X|Y}(x|2) &=\frac{x^2(1-x)^2}{\int_0^1 x^2(1-x)^2 dx} \\
& = 30 x^2(1-x)^2
\end{align*}
for $0\le x \le1$ and 0 otherwise.  As a sanity check, I made sure the posterior integrates to 1.

\end{problem}

\begin{problem}{2} From Baye's rule we know that the posterior density is:
\begin{equation*}
f_{X|Y}(x|5) \propof{x} P_{Y|X}(5|x)f_X(x) = 3x^3(1-x)^4,
\end{equation*}
where the symbol $\propof{x}$ means proportional to as a function of $x$.  Therefore, the MAP estimate is given by
\begin{equation*}
\hat x_{MAP} = \argmax_{x \in [0, 1]}  \{3x^3(1-x)^4 \},
\end{equation*}
which can be found setting the derivative of the argument equal to zero and solving for $x$:
\begin{equation*}
0 = 9\hat x_{MAP}^2(1-\hat x_{MAP})^4-12\hat x_{MAP}^3(1-\hat x_{MAP})^3
\end{equation*}
$\implies$ $\hat x_{MAP} = 3/7$, which is indeed in the interval $[0, 1]$


\end{problem}

\begin{problem}{3}  The conditional PDF of $X|Y$ is given by
\begin{equation*}
f_{X|Y}(x|y) = \frac{f_{XY}(x,y)}{f_{Y}(y)} \propof{x} f_{XY}(x,y),
\end{equation*}
so that the MAP estimate of $x$ is:
\begin{equation*}
\hat x_{MAP} = \argmax_{x \in [0, 1]} \{ f_{XY}(x,y)\}.
\end{equation*}
On the other hand, the conditional PDF of $Y|X$ is given by
\begin{equation*}
f_{Y|X}(y|x) = \frac{f_{XY}(x,y)}{f_{X}(x)} = \frac{f_{XY}(x,y)}{\int f_{XY}(x,y)dy}, 
\end{equation*}
so that the ML estimate of $x$ is:
\begin{equation*}
\hat x_{ML} = \argmax_{x \in [0, 1]}\left  \{ \frac{f_{XY}(x,y)}{\int f_{XY}(x,y)dy} \right \}.
\end{equation*}

Since the joint PDF is
\[
  f_{XY}(x,y) =
  \begin{cases}
                                   x+\frac{3}{2}y^2 & \text{for $0 \le x,y\le 1$} \\
                                   0 & \text{otherwise},
  \end{cases}
\]
we see that $ f_{XY}(x,y)$ is maximized when $x = 1$, and therefore $\hat x_{MAP} = 1$.

From the equation above:
\begin{align*}
f_{Y|X}(y|x) &=\frac{x+\frac{3}{2}y^2}{\int x+\frac{3}{2}y^2dy} \\
& = \frac{2x+3y^2}{2x+1} \\
&=1+\frac{3y^2-1}{2x+1}
\end{align*},
and thus we see that, to maximize this expression, if $3y^2-1\le 0$ we need to minimize the second term, while if $3y^2-1> 0$ we need to maximize it.  Therefore:
\[
  \hat x_{ML} =
  \begin{cases}
                                   1 & \text{for $y \le \frac{1}{\sqrt{3}}$} \\
                                   0 & \text{otherwise}.
  \end{cases}
\]


\end{problem}


\begin{problem}{4} The posterior distribution is:

\begin{align*}
f_{X|Y}(x|y) &= \frac{f_{X|Y}(x|y) f_{X}(x)}{\int f_{X|Y}(x|y) f_{X}(x) dx} \\
& = \frac{(xy- \frac{x}{2}+1)(2x^2+\frac{1}{3})}{\int_0^1 (xy- \frac{x}{2}+1)(2x^2+\frac{1}{3}) dx}\\
& = \frac{2x^3y+\frac{xy}{3}-x^3-\frac{x}{6}+2x^2+\frac{1}{3}}{\frac{2}{3}y+\frac{1}{2}},
\end{align*} 
so that
\begin{align*}
\hat x_M &= E[X|Y=y]\\
& = \frac{1}{\frac{2}{3}y+\frac{1}{2}} \int_0^1 \left (2x^4y+\frac{x^2y}{3}-x^4-\frac{x^2}{6}+2x^3+\frac{x}{3} \right)dx \\
& = \frac{23}{45}y+\frac{37}{90}.
\end{align*} 

\end{problem}










